Maps/Maps.dfy
@@ -18,9 +18,7 @@ module Maps {
 	  imap x | x in m :: m[x]
 	}
 
-  /**
-   * Remove all key-value pairs corresponding to the set of keys provided.
-   */
+  /* Remove all key-value pairs corresponding to the set of keys provided. */
   function method {:opaque} remove_keys<X, Y>(m: map<X, Y>, xs: set<X>): (m': map<X, Y>)
     ensures forall x {:trigger m'[x]} :: x in m && x !in xs ==> x in m' && m'[x] == m[x]
     ensures forall x {:trigger x in m'} :: x in m' ==> x in m && x !in xs
@@ -29,9 +27,7 @@ module Maps {
     map x | x in m && x !in xs :: m[x]
   }
 
-  /**
-   * Remove a key-value pair. Returns unmodified map if key is not found.
-   */
+  /* Remove a key-value pair. Returns unmodified map if key is not found. */
   function method {:opaque} remove<X, Y>(m: map<X, Y>, x: X): (m': map<X, Y>)
     ensures m' == remove_keys(m, {x})
     ensures |m'.Keys| <= |m.Keys|
@@ -43,36 +39,29 @@ module Maps {
     m'
   }
 
-  /**
-   * Keep all key-value pairs corresponding to the set of keys provided.
-   */
+  /* Keep all key-value pairs corresponding to the set of keys provided. */
   function method {:opaque} restrict<X, Y>(m: map<X, Y>, xs: set<X>): (m': map<X, Y>)
     ensures m' == remove_keys(m, m.Keys - xs)
   {
     map x | x in xs && x in m :: m[x]
   }
 
-  /**
-   * True iff two maps contain the same key-value pairs for intersecting keys.
-   */
+  /* True iff two maps contain the same key-value pairs for intersecting
+  keys. */
   predicate equal_on_key<X, Y>(m: map<X, Y>, m': map<X, Y>, x: X)
   {
     (x !in m && x !in m') || (x in m && x in m' && m[x] == m'[x])
   }
 
-  /**
-   * True iff m is a subset of m'.
-   */
+  /* True iff m is a subset of m'. */
   predicate is_subset<X, Y>(m: map<X, Y>, m': map<X, Y>)
   {
     && m.Keys <= m'.Keys
     && forall x {:trigger equal_on_key(m, m', x)}{:trigger x in m} :: x in m ==> equal_on_key(m, m', x)
   }
 
-  /**
-   * Union of two maps. Does not require disjoint domains; on the intersection,
-   * values from the first map are chosen.
-   */
+  /* Union of two maps. Does not require disjoint domains; on the intersection,
+  values from the first map are chosen. */
   function method {:opaque} union<X, Y>(m: map<X, Y>, m': map<X, Y>): (r: map<X, Y>)
     ensures r.Keys == m.Keys + m'.Keys
     ensures forall x {:trigger r[x]} :: x in m ==> r[x] == m[x]
@@ -81,9 +70,8 @@ module Maps {
     map x | x in m.Keys + m'.Keys :: if x in m then m[x] else m'[x]
   }
 
-  /**
-   * The size of the disjoint union is equal to the sum of individual map sizes.
-   */
+  /* The size of the disjoint union is equal to the sum of individual map
+  sizes. */
   lemma lemma_disjoint_union_size<X, Y>(m: map<X, Y>, m': map<X, Y>)
     requires m.Keys !! m'.Keys
     ensures |union(m, m')| == |m| + |m'|
@@ -92,26 +80,20 @@ module Maps {
     assert |u.Keys| == |m.Keys| + |m'.Keys|;
   }
 
-  /**
-   * True iff a map is injective.
-   */
+  /* True iff a map is injective. */
   predicate {:opaque} injective<X, Y>(m: map<X, Y>)
   {
     forall x, x' {:trigger m[x], m[x']} :: x != x' && x in m && x' in m ==> m[x] != m[x']
   }
 
-  /**
-   * Swaps map keys and values. Values are not required to be unique; no
-   * promises on which key is chosen on the intersection.
-   */
+  /* Swaps map keys and values. Values are not required to be unique; no
+  promises on which key is chosen on the intersection. */
   function {:opaque} invert<X, Y>(m: map<X, Y>): map<Y, X>
   {
     map y | y in m.Values :: var x :| x in m.Keys && m[x] == y; x
   }
 
-  /**
-   * Inverted maps are injective.
-   */
+  /* Inverted maps are injective. */
   lemma lemma_invert_is_injective<X, Y>(m: map<X, Y>)
     ensures injective(invert(m))
   {
@@ -119,26 +101,20 @@ module Maps {
     reveal_invert();
   }
 
-  /**
-   * True iff a map contains all valid keys.
-   */
+  /* True iff a map contains all valid keys. */
   predicate {:opaque} total<X(!new), Y>(m: map<X, Y>)
   {
     forall i {:trigger m[i]}{:trigger i in m} :: i in m
   }
 
-  /**
-   * True iff a map is monotonic.
-   */
+  /* True iff a map is monotonic. */
   predicate {:opaque} monotonic(m: map<int, int>)
   {
     forall x, x' {:trigger m[x], m[x']} :: x in m && x' in m && x <= x' ==> m[x] <= m[x']
   }
 
-  /**
-   * True iff a map is monotonic. Only considers keys greater than or
-   * equal to start.
-   */
+  /* True iff a map is monotonic. Only considers keys greater than or
+  equal to start. */
   predicate {:opaque} monotonic_from(m: map<int, int>, start: int)
   {
     forall x, x' {:trigger m[x], m[x']} :: x in m && x' in m && start <= x <= x' ==> m[x] <= m[x']
