Sets/Isets.dfy
@@ -4,18 +4,14 @@ module Isets {
 
   import Math = Mathematics
 
-  /**
-   * If all elements in iset x are in iset y, x is a subset of y.
-   */
+  /* If all elements in iset x are in iset y, x is a subset of y. */
   lemma lemma_subset<T>(x: iset<T>, y: iset<T>)
     requires forall e {:trigger e in y} :: e in x ==> e in y
     ensures x <= y
   {
   }
 
-  /**
-   * Apply an injective function to each element of an iset.
-   */
+  /* Apply an injective function to each element of an iset. */
   function {:opaque} apply<X(!new), Y>(xs: iset<X>, f: X-->Y): (ys: iset<Y>)
     reads f.reads
     requires forall x {:trigger f.requires(x)} :: f.requires(x)
@@ -26,10 +22,8 @@ module Isets {
     ys
   }
 
-  /**
-   * Construct an iset using elements of another set for which a function returns
-   * true.
-   */
+  /* Construct an iset using elements of another set for which a function
+  returns true. */
   function {:opaque} filter<X(!new)>(xs: iset<X>, f: X~>bool): (ys: iset<X>)
     reads f.reads
     requires forall x {:trigger f.requires(x)} {:trigger x in xs} :: x in xs ==> f.requires(x)
